wip: sponge functions

src/lib.rs
@@ -1,4 +1,5 @@
 pub mod simple;
+mod foo;
 
 pub fn get_vec_of_bits(s: &str) -> Vec<bool> {
     let mut res = vec![];
