lean/Shars/Verification/Simple/Sponge.lean
@@ -1,0 +1,242 @@
+import Aeneas
+import Shars.BitVec
+import Shars.ArrayExtract
+import Shars.Definitions.Simple
+import Sha3.Spec
+import Aeneas.SimpLists.Init
+import Sha3.Facts
+import Init.Data.Vector.Lemmas
+import Init.Data.Nat.Basic
+import Init.Data.Array
+import Shars.Verification.Simple.Utils
+import Shars.Verification.Simple.Auxiliary
+import Shars.Verification.Simple.KeccakP
+
+set_option maxHeartbeats 1000000
+attribute [-simp] List.getElem!_eq_getElem?_getD
+attribute [simp] Aeneas.Std.Slice.set
+
+open Aeneas hiding Std.Array
+open Std.alloc.vec 
+
+abbrev spec_sponge (r: Nat)(r_pos: r > 0):= 
+  have: NeZero r := ⟨Nat.not_eq_zero_of_lt r_pos⟩
+  Spec.sponge (f := Spec.Keccak.P 6 24) (pad := Spec.«pad10*1»)
+abbrev spec_sponge_absorb (r: Nat)(r_pos: r > 0) := 
+  have: NeZero r := ⟨Nat.not_eq_zero_of_lt r_pos⟩
+  Spec.sponge.absorb (f := Spec.Keccak.P 6 24) (pad := Spec.«pad10*1») (r := r) 
+abbrev spec_sponge_squeze{m d}(r: Nat)(r_pos: r > 0) := 
+  have: NeZero r := ⟨Nat.not_eq_zero_of_lt r_pos⟩
+  Spec.sponge.squeeze (m := m) (d := d) (f := Spec.Keccak.P 6 24) (r := r)
+
+def Vector.toBitVec(self: Vector Bool n): BitVec n := (BitVec.ofBoolListLE <| self.toList).cast (by simp)
+
+def absorb{r: Nat}(S: BitVec (Spec.b 6))(Ps: Array (BitVec r)) := Id.run do
+  let mut S := S
+  for P in Ps do
+    S := Spec.Keccak.P 6 24 (S ^^^ P.setWidth (Spec.b 6))
+  return S
+
+theorem absorb.spec (N : Array Spec.Bit) (r: Nat)(r_pos: r > 0)
+: spec_sponge_absorb r r_pos N = absorb (0#(Spec.b 6)) ((N ++ Spec.«pad10*1» r N.size).chunks_exact r |>.map (·.toBitVec))
+:= by sorry
+
+@[elab_as_elim, cases_eliminator]
+def Array.cases_extract(k: Nat)[NeZero k]
+  {motive : Array α → Prop}
+  (onSmall: (rest: Array α) → (small: rest.size < k) → motive rest)
+  (onBig: (chunk: Vector α k) → (rest: Array α) → motive (chunk.toArray ++ rest))
+  (arr: Array α)
+: motive arr
+:= 
+  if h: arr.size < k then
+    onSmall arr h
+  else
+    let chunk: Vector α k := ⟨arr.extract (stop  := k), (by simpa using h)⟩
+    let other := arr.extract (start := k)
+    have properPartition: chunk.toArray ++ other = arr := by simp [chunk, other]
+    properPartition ▸ onBig chunk other
+
+@[simp]
+theorem Array.size_chunks_exact[Inhabited α](arr: Array α)(k: Nat)
+: (arr.chunks_exact k).size = arr.size / k
+:= by
+  rw [chunks_exact]
+  split
+  case isTrue h =>
+    rcases h with arr_small | k_zero
+    · simp [Nat.div_eq_of_lt arr_small]
+    · simp [k_zero]
+  case isFalse h =>
+    simp at h
+    obtain ⟨k_lt_size, k_pos⟩ := h
+    simp
+    have ih: (chunks_exact k (arr.extract k)).size = (arr.size - k) / k
+      := by simpa using (arr.extract k).size_chunks_exact k
+    rw [
+      ih, 
+      Nat.add_comm,
+      ←Nat.add_div_right (H := Nat.zero_lt_of_ne_zero k_pos),
+      Nat.sub_add_cancel k_lt_size
+    ]
+termination_by arr.size
+decreasing_by 
+  replace k_pos := Nat.zero_lt_of_ne_zero k_pos
+  simp [k_pos]
+  apply trans k_pos k_lt_size
+
+theorem Array.extract_start_start(arr: Array α)(start: Nat)
+: arr.extract start start = #[]
+:= by simp only [extract_eq_empty_iff, inf_le_left]
+
+theorem Array.getElem_chunks_exact[Inhabited α](arr: Array α)(k i: Nat)(i_idx: i < arr.size / k)
+: k > 0 
+→ (arr.chunks_exact k)[i]!.toArray = arr.extract (k*i) (k*(i+1))
+:= by
+  intro k_pos
+  have: NeZero k := {out := by omega}
+  have : i < (chunks_exact k arr).size := by simp [i_idx]
+  rw [getElem!_pos _ i this]
+
+  cases arr using Array.cases_extract k
+  case onSmall small =>
+    have: arr.size / k = 0 := Nat.div_eq_of_lt small
+    simp [this] at i_idx
+  case onBig chunk rest =>
+    /- rw [Array.chunks_exact] -- TODO: Why does rw fail here? -/
+    unfold Array.chunks_exact
+    simp [Nat.not_eq_zero_of_lt k_pos, Array.extract_start_start]
+    cases i
+    case zero =>
+      simp
+      rw [Array.getElem_append_left (Nat.one_pos)]
+      simp
+    case succ i' =>
+      rw [Array.getElem_append_right (by simp)]
+      simp 
+      rw [getElem_eq_getElem!]
+
+      rw [Array.extract_empty_of_size_le_start chunk.toArray (by simp)]
+      rw [Array.extract_empty_of_size_le_start chunk.toArray ?precond]
+      case precond => simp; (conv => arg 1; rw [←Nat.mul_one k]); apply Nat.mul_le_mul_left; simp
+
+      simp
+      have ih := Array.getElem_chunks_exact rest k i'
+      rw [ih ?i_idx (k_pos)]
+      case i_idx => simpa [Nat.add_div_left (H := k_pos)] using i_idx
+
+      ring_nf
+      congr
+      · rw[Nat.add_comm, Nat.add_sub_cancel]
+      · rw[Nat.add_comm (k*2), Nat.mul_two, ←Nat.add_assoc, Nat.add_sub_cancel, Nat.add_comm]
+
+
+def Aeneas.Std.Array.toArray{size: Usize}(self: Aeneas.Std.Array α size): _root_.Array α := Array.mk self.val
+def Aeneas.Std.Slice.toArray(self: Aeneas.Std.Slice α): _root_.Array α := Array.mk self.val
+
+/- @[progress] -/
+/- theorem Aeneas.Std.core.slice.index.Slice.index.spec -/
+/-   (bs: Std.Slice α)(inst: SliceIndex (ops.range.Range Usize) (Slice α) (Slice α))(range: ops.range.Range Usize) -/
+/- : ∃ output, -/
+/-   Aeneas.Std.core.slice.index.Slice.index inst bs range = .ok output ∧ -/
+
+
+/-     (Std.core.slice.index.SliceIndexRangeUsizeSliceInst Bool) bs := -/ 
+
+attribute [simp] Aeneas.Std.core.slice.index.Slice.index
+
+@[progress]
+theorem Aeneas.Std.core.slice.index.SliceIndexRangeUsizeSlice.index.spec(input: Slice α)(r: ops.range.Range Usize)
+: r.start.val ≤ r.end_.val
+→ r.end_.val ≤ input.length
+→ ∃ output,
+  core.slice.index.SliceIndexRangeUsizeSlice.index r input = .ok output ∧
+  output.val = input.val.extract r.start.val r.end_.val
+:= by
+  obtain ⟨start, end_⟩ := r
+  intro r_proper end_lt_length
+  simp at *
+  rw [index]
+  simp [List.slice, *]
+
+@[progress]
+theorem Aeneas.Std.core.slice.index.Slice.index.slice_index_range_usize_slice_spec(input: Slice α)(r: ops.range.Range Usize)
+: r.start.val ≤ r.end_.val
+→ r.end_.val ≤ input.length
+→ ∃ output,
+  core.slice.index.Slice.index (Std.core.slice.index.SliceIndexRangeUsizeSliceInst α) input r = .ok output ∧
+  output.val = input.val.extract r.start.val r.end_.val
+:= by simpa using SliceIndexRangeUsizeSlice.index.spec input r
+
+
+@[progress]
+theorem simple.sponge_absorb_initial_loop.spec
+  (bs : Std.Slice Bool) (r : Std.Usize) (s : Aeneas.Std.Array Bool 1600#usize) (n i : Std.Usize)
+: n.val = bs.length / r.val
+→ (r_pos: r.val > 0)
+→ ∃ output,
+  sponge_absorb_initial_loop bs r s n i = .ok output ∧ 
+  have h: (1600#usize).val = Spec.b 6 := by simp [Spec.w, Spec.b]
+  output.toBitVec = ((absorb (s.toBitVec.cast h) (bs.toArray.chunks_exact r |>.map (·.toBitVec) |>.drop i)).cast h.symm)
+:= by
+  rintro n_val r_pos
+  rw [sponge_absorb_initial_loop]
+  split
+  . let* ⟨ i1, i1_post ⟩ ← Std.Usize.mul_spec
+    · sorry
+    let* ⟨ i2, i2_post ⟩ ← Std.Usize.add_spec
+    let* ⟨ i3, i3_post ⟩ ← Std.Usize.mul_spec
+    · sorry
+    let* ⟨ slice, slice_post ⟩ ← Std.core.slice.index.Slice.index.slice_index_range_usize_slice_spec
+    · sorry
+    let* ⟨old_slice, new_slice⟩ ← Std.Array.to_slice_mut.progress_spec
+    let* ⟨ s2, s2_post ⟩ ← xor_long.spec
+    let* ⟨ s4, s4_post ⟩ ← keccak_p.spec
+    let* ⟨_, _ ⟩ ← spec
+    simp [*]
+    sorry
+
+  case isFalse h =>
+    have := ‹bs.length / r.val - i.val = 0›'
+    simp [absorb, this]
+    sorry
+
+
+/- @[progress] -/
+theorem simple.sponge_absorb_initial.spec
+  (bs : Std.Slice Bool) (r : Std.Usize) (s : Aeneas.Std.Array Bool _)
+(r_pos: r.val > 0)
+: s.toBitVec = (0#(Spec.b 6)).cast (by simp [Spec.w, Spec.b])
+→ ∃ output,
+  sponge_absorb_initial bs r s = .ok output ∧ 
+  output.toBitVec = ((spec_sponge_absorb r.val r_pos ⟨bs.val⟩).cast (by simp [Spec.w, Spec.b]))
+:= by sorry
+
+/- @[progress] -/
+theorem simple.sponge_absorb_final.spec
+  (rest suffix : Std.Slice Bool) (r : Std.Usize) (s : Aeneas.Std.Array Bool _)
+(r_pos: r.val > 0)
+: ∃ output,
+  sponge_absorb_final s rest suffix r = .ok output ∧ 
+  output.toBitVec = (spec_sponge_absorb r.val r_pos ⟨bs.val⟩).cast (by simp [Spec.w, Spec.b]))
+:= by sorry
+
+
+/- @[progress] -/
+theorem simple.sponge_absorb.spec
+  (bs : Std.Slice Bool) (r : Std.Usize) [NeZero r.val](output : Aeneas.Std.Array Bool 1600#usize)
+  (suffix : Std.Slice Bool)
+: ∃ output,
+  sponge_absorb_initial_loop
+  sponge_absorb bs r output suffix = .ok output ∧
+  output.val = (Spec.sponge.absorb (f:=Spec.Keccak.P 6 24) (pad:=Spec.«pad10*1») r.val (Array.mk <| bs.val ++ suffix.val)).toArray.toList
+:= by sorry
+
+-- @[progress]
+theorem simple.sponge.spec (r : Std.Usize) (bs output suffix: Std.Slice Bool) 
+[NeZero r.val]
+/- (r_ne_zero: r.val ≠ 0) -/
+: ∃ output,
+  simple.sponge r bs output suffix = .ok output ∧
+  output.val = (Spec.sponge (f := Spec.Keccak.P 6 (nᵣ := 24)) (pad := Spec.«pad10*1») r.val (Array.mk <| bs.val ++ suffix.val ) output.length).toArray.toList
+:= by sorry
